@prefix afn:     <http://jena.hpl.hp.com/ARQ/function#> .
@prefix :        <http://purl.obolibrary.org/obo/arg/app-views/vivo/vivo-app.owl#> .
@prefix hr:      <http://vivo.cornell.edu/ns/hr/0.9/hr.owl#> .
@prefix ns:      <http://www.w3.org/2003/06/sw-vocab-status/ns#> .
@prefix scires:  <http://vivoweb.org/ontology/scientific-research#> .
@prefix aka:     <http://vivoweb.org/ontology/aka#> .
@prefix scirr:   <http://vivoweb.org/ontology/scientific-research-resource#> .
@prefix vann:    <http://purl.org/vocab/vann/> .
@prefix pubmed:  <http://vitro.mannlib.cornell.edu/ns/pubmed#> .
@prefix owl2:    <http://www.w3.org/2006/12/owl2-xml#> .
@prefix dcterms:  <http://purl.org/dc/terms/> .
@prefix rdfs:    <http://www.w3.org/2000/01/rdf-schema#> .
@prefix swrl:    <http://www.w3.org/2003/11/swrl#> .
@prefix vitro:   <http://vitro.mannlib.cornell.edu/ns/vitro/0.7#> .
@prefix event:   <http://purl.org/NET/c4dm/event.owl#> .
@prefix vivoc:   <http://vivo.library.cornell.edu/ns/0.1#> .
@prefix swvs:    <http://www.w3.org/2003/06/sw-vocab-status/ns#> .
@prefix rdf:     <http://www.w3.org/1999/02/22-rdf-syntax-ns#> .
@prefix c4o:     <http://purl.org/spar/c4o/> .
@prefix cce:     <http://vivoweb.org/ontology/cornell-cooperative-extension#> .
@prefix vivo:    <http://vivoweb.org/ontology/core#> .
@prefix dcelem:  <http://purl.org/dc/elements/1.1/> .
@prefix app:     <http://eagle-i.org/ont/app/1.0/> .
@prefix pvs:     <http://vivoweb.org/ontology/provenance-support#> .
@prefix geo:     <http://aims.fao.org/aos/geopolitical.owl#> .
@prefix foaf:    <http://xmlns.com/foaf/0.1/> .
@prefix aktp:    <http://www.aktors.org/ontology/portal#> .
@prefix far:     <http://vitro.mannlib.cornell.edu/ns/reporting#> .
@prefix fabio:   <http://purl.org/spar/fabio/> .
@prefix skco:    <http://www.w3.org/2004/02/skos/core#> .
@prefix ospcu:   <http://vivoweb.org/ontology/cu-vivo-osp#> .
@prefix acti:    <http://vivoweb.org/ontology/activity-insight#> .
@prefix obo:     <http://purl.obolibrary.org/obo/> .
@prefix skos2:   <http://www.w3.org/2008/05/skos#> .
@prefix stars:   <http://vitro.mannlib.cornell.edu/ns/cornell/stars/classes#> .
@prefix bibo:    <http://purl.org/ontology/bibo/> .
@prefix xsd:     <http://www.w3.org/2001/XMLSchema#> .
@prefix swrlb:   <http://www.w3.org/2003/11/swrlb#> .
@prefix owl:     <http://www.w3.org/2002/07/owl#> .
@prefix socsci:  <http://vivo.library.cornell.edu/ns/vivo/socsci/0.1#> .
@prefix rdfsyn:  <http://www.w3.org/1999/02/22-rdf-syntax-ns#> .
@prefix core:    <http://vivoweb.org/ontology/core#> .
@prefix vitro-public:  <http://vitro.mannlib.cornell.edu/ns/vitro/public#> .
@prefix local:   <http://vivo.cornell.edu/ontology/local#> .
@prefix mann:    <http://vivo.cornell.edu/ns/mannadditions/0.1#> .
@prefix skos:    <http://www.w3.org/2004/02/skos/core#> .
@prefix ero:     <http://purl.obolibrary.org/obo/> .

core:FacultyMember
      a       owl:Class ;

      rdfs:subClassOf foaf:Person ;
      vitro:descriptionAnnot
              "Definition from here: http://research.carleton.ca/htr/defs.php."^^xsd:string ;
      obo:IAO_0000115 "A person with at least one academic appointment to a specific faculty of a university or institution of higher learning."^^xsd:string .

core:Postdoc
      a       owl:Class ;

      rdfs:subClassOf core:NonFacultyAcademic ;
      obo:IAO_0000115 "A Person holding an academic employment appointment focused on research rather than teaching; temporary (or for some defined term)"^^xsd:string .

core:NonFacultyAcademic
      a       owl:Class ;

      rdfs:subClassOf foaf:Person ;
      obo:IAO_0000115 "A person not considered a faculty member but holding an academic appointment."^^xsd:string .

core:EmeritusLibrarian
      a       owl:Class ;

      rdfs:subClassOf foaf:Person ;
      obo:IAO_0000115 "A retired librarian who has retained their rank, title and privileges."^^xsd:string .

core:EmeritusFaculty
      a       owl:Class ;

      rdfs:subClassOf foaf:Person ;
      obo:IAO_0000115 "A retired faculty member who has retained their rank, title and privileges."^^xsd:string .

core:Librarian
      a       owl:Class ;

      rdfs:subClassOf foaf:Person ;
      obo:IAO_0000115 "A person working in a position of librarian or information professional, or academic or technical expert in support of providing information services or materials."^^xsd:string .

core:EmeritusProfessor
      a       owl:Class ;

      rdfs:subClassOf core:EmeritusFaculty , foaf:Person ;
      obo:IAO_0000115 "A retired professor who has retained their rank, title and privileges."^^xsd:string .

core:NonAcademic
      a       owl:Class ;

      rdfs:subClassOf foaf:Person ;
      obo:IAO_0000115 "A person holding a position that is not considered to be an academic appointment."^^xsd:string .
